\chapter{Svolgimento completo esercizio 5.4}

	\begin{align*}
		\sssssssvar & = (\lambda xyz.xz(yz))\ssssssvar\\
		& = (\lambda yz.\svar z(yz))\sssssvar\\
		& = (\lambda z.\svar z(\svar z))\ssssvar\\
		& = \ssvar(\ssvar)\sssvar\\
		& = (\lambda yz.\svar z(yz))(\ssvar)\sssvar\\
		& = (\lambda z.\svar z(\ssvar)z)\sssvar\\
		& = \ssvar(\sssvar)\ssvar\\
		& = (\lambda yz.\svar z(yz))(\sssvar)\ssvar\\
		& = (\lambda z.\svar z(\sssvar z))\ssvar\\
		& = \ssvar(\ssssvar)\svar\\
		& = (\lambda yz.\svar z(yz))(\ssssvar)\svar\\
		& = (\lambda z.\svar z(\ssssvar z))\svar\\
		& = \ssvar(\sssssvar)\\
		& = (\lambda yz.\svar z(yz))(\sssssvar)\\
		& = \lambda z.\svar z(\sssssvar z)\\
		& = \lambda z.(\lambda ya.a (y a))(\sssssvar z)\\
		& = \lambda za.a a(\sssssvar a a)\\
		& = \lambda za.a a((\lambda yb.\svar b (y b)) \sssvar z z)\\
		& = \lambda za.a a((\lambda b.\svar b(\svar b))\svar \svar z z)\\
		& = \lambda za.a a(\svar \svar(\svar \svar)\svar a a)\\
		& = \lambda za.a a((\lambda yb.\svar b(y b))\sssvar z z)\\
		& = \lambda za.a a((\lambda b.\svar b(\svar b))\ssvar z z)\\
		& = \lambda za.a a(\svar \svar(\ssvar )\svar a a)\\
	\end{align*}
	\begin{align*}
		& = \lambda za.a a((\lambda yb.\svar b(y b))(\ssvar )\svar z z)\\
		& = \lambda za.a a((\lambda b.\svar b(\ssvar b))\svar z z)\\
		& = \lambda za.a a(\svar \svar(\sssvar)a a)\\
		& = \lambda za.a a((\lambda yb.\svar b(y b))(\sssvar)z z)\\
		& = \lambda za.a a((\lambda b.\svar b(\sssvar b))z z)\\
		& = \lambda za.a a(\svar a(\sssvar a)a)\\
		& = \lambda za.a a((\lambda yb.b b(y b))(\sssvar z)\\
		& = \lambda za.a a((\lambda b.b b(\sssvar b b))z)\\
		& = \lambda za.a a(a a(\sssvar a))\\
		& = \lambda za.a a(a a((\lambda yb.\svar b(y b))\svar z z))\\
		& = \lambda za.a a(a a (\svar a(\svar a)a))\\
		& = \lambda za.a a(a((\lambda yb.b b(y b))(\svar z)z))\\
		& = \lambda za.a a(a a((\lambda b.b b(\svar b b))z))\\
		& = \lambda za.a a(a a(a a(\svar a a)))\\
		& = \lambda za.a a(a a(a a((\lambda yb.b b(y b))z)))\\
		& = \lambda za.a a(a a(a a(\lambda b.b b(b b))))\\
	\end{align*}